pulse/Pulse.Lib.C.Palow.Aggregate.fst
@@ -115,12 +115,12 @@ ghost fn struct_S_split (a: ptr) (#p: perm) (#x: struct_S)
 
   mem_split a 4sz;
   Seq.lemma_eq_intro (slice b 0 4) (encode 4 None (U32.v x.f));
-  fold uint32_t_pts_to a p x.f;
+  uint32_t_conceal a #p #_ #x.f;
 
   mem_split (a +! 4sz) 1sz;
   Seq.slice_slice b 4 8 0 1;
   Seq.lemma_eq_intro (slice (slice b 4 (len b)) 0 1) (encode 1 None (U8.v x.g));
-  fold uint8_t_pts_to (a +! struct_S_offsetof_g) p x.g;
+  uint8_t_conceal (a +! struct_S_offsetof_g) #p #_ #x.g;
 
   Seq.slice_slice b 4 8 1 4;
   struct_S_padptr a;
@@ -138,8 +138,8 @@ ghost fn struct_S_join (a: ptr) (#p: perm) (#x: struct_S)
   requires struct_S_padding a p
   ensures  struct_S_pts_to a p x
 {
-  unfold uint32_t_pts_to a p x.f;
-  unfold uint8_t_pts_to (a +! struct_S_offsetof_g) p x.g;
+  uint32_t_reveal a #p #x.f;
+  uint8_t_reveal (a +! struct_S_offsetof_g) #p #x.g;
   unfold struct_S_padding a p;
   with pad. assert (mem_pts_to (a +! struct_S_padoff) p pad);
 
@@ -208,8 +208,8 @@ ghost fn struct_T_split (a: ptr) (#p: perm) (#x: struct_T)
   mem_split a 4sz;
   Seq.lemma_eq_intro (slice b 0 4) (encode 4 None (U32.v x.y));
   Seq.lemma_eq_intro (slice b 4 (len b)) (encode 4 None (U32.v x.z));
-  fold uint32_t_pts_to a p x.y;
-  fold uint32_t_pts_to (a +! struct_T_offsetof_z) p x.z;
+  uint32_t_conceal a #p #_ #x.y;
+  uint32_t_conceal (a +! struct_T_offsetof_z) #p #_ #x.z;
 }
 
 ghost fn struct_T_join (a: ptr) (#p: perm) (#x: struct_T)
@@ -217,8 +217,8 @@ ghost fn struct_T_join (a: ptr) (#p: perm) (#x: struct_T)
   requires uint32_t_pts_to (a +! struct_T_offsetof_z) p x.z
   ensures  struct_T_pts_to a p x
 {
-  unfold uint32_t_pts_to a p x.y;
-  unfold uint32_t_pts_to (a +! struct_T_offsetof_z) p x.z;
+  uint32_t_reveal a #p #x.y;
+  uint32_t_reveal (a +! struct_T_offsetof_z) #p #x.z;
   rewrite (mem_pts_to (a +! struct_T_offsetof_z) p (encode 4 None (U32.v x.z)))
        as (mem_pts_to (a +! 4sz) p (encode 4 None (U32.v x.z)));
   mem_join a #p #(encode 4 None (U32.v x.y)) #(encode 4 None (U32.v x.z)) 4sz;
@@ -259,14 +259,14 @@ ghost fn uint32_t_of_elem (a: ptr) (#p: perm) (#x: U32.t)
   ensures  uint32_t_pts_to a p x
 {
   unfold elem_pts_to uint32_t_repr a p x;
-  fold uint32_t_pts_to a p x;
+  uint32_t_conceal a #p #_ #x;
 }
 
 ghost fn uint32_t_to_elem (a: ptr) (#p: perm) (#x: U32.t)
   requires uint32_t_pts_to a p x
   ensures  elem_pts_to uint32_t_repr a p x
 {
-  unfold uint32_t_pts_to a p x;
+  uint32_t_reveal a #p #x;
   fold elem_pts_to uint32_t_repr a p x;
 }
 
